theories/tree_borrows/step_laws/steps_refl.v
@@ -180,15 +180,15 @@ Proof.
   specialize (pool_safe_implies Hsafe Hpool) as (trs' & Hdealloc_s & Hpos & Hcontain & Happly_s).
   iPoseProof (bor_interp_get_pure with "Hbor") as "%Hp".
   destruct Hp as (Hsst_eq & Hsnp_eq & Hsnc_eq & Hscs_eq & Hwf_s & Hwf_t & Hdom_eq).
-  odestruct (apply_within_trees_equal _ _ _ _ _ _ _ Happly_s) as (trt' & Happly_t & Heq'); [|exact Hsst_eq|].
+  odestruct (apply_within_trees_equal _ _ _ _ _ _ _ _ Happly_s) as (trt' & Happly_t & Heq'); [|exact Hsst_eq|].
   { intros ttr1 ttr1' ttr2 H1 H2 Httr1 Httr1' Httr2.
     assert (tree_contains bor_s ttr1) as Hcont' by rewrite /trees_contain /trees_at_block Httr1 // in Hcontain.
-    edestruct tree_equal_allows_more_deallocation as (ttr2'&Httr2').
-    1,3,4,6: by eapply Hwf_s. 1: by eapply Hwf_t. 1: eapply H2.
+    edestruct tree_equal_allows_more_deallocation as (ttr2'&Httr2'). 9: exact H2.
+    1,5,6: by eapply Hwf_s. 1-5: rewrite ?Hscs_eq; by eapply Hwf_t. 1: by eapply Hwf_s.
     1: eapply mk_is_Some, H1.
     exists ttr2'; split; first done.
-    eapply tree_equal_memory_deallocate. 5,6,4,3: done.
-    all: eapply wf_tree_tree_unique. 1: by eapply Hwf_s. by eapply Hwf_t. }
+    eapply tree_equal_memory_deallocate. 7-10: done.
+    1,3,4: by eapply Hwf_s. 3: rewrite Hscs_eq. all: by eapply Hwf_t. }
   iSplitR.
   { iPureIntro. do 3 eexists. eapply dealloc_base_step'; try done.
     - setoid_rewrite <- elem_of_dom. setoid_rewrite <- elem_of_dom in Hdealloc_s. rewrite -Hdom_eq //.
@@ -399,7 +399,7 @@ Proof.
   destruct Hp as (Hstrs_eq & Hsnp_eq & Hsnc_eq & Hscs_eq & Hwf_s & Hwf_t & Hdom_eq).
   specialize (pool_safe_implies Hsafe Hpool) as (?&[= <-]&Hcall_in & trss' & Htrss).
   edestruct trees_equal_access_all_protected_initialized as (trst' & Htrst & Htrseq').
-  11: exact Hstrs_eq. 5,7: rewrite Hscs_eq. 11: exact Htrss. 1,3,4,7,8: by eapply Hwf_s. 4: rewrite Hsnp_eq Hsnc_eq. 1-4: by eapply Hwf_t. 1: done.
+  13: exact Hstrs_eq. 7,9: rewrite Hscs_eq. 13: exact Htrss. 1,4,6,9,10: by eapply Hwf_s. 6: rewrite Hsnp_eq Hsnc_eq. 1-6: by eapply Hwf_t. 1: done.
   iSplit.
   { iPureIntro. do 3 eexists. eapply end_call_base_step. all: by rewrite -Hscs_eq. }
   iIntros (e_t' efs_t σ_t') "%Hhead".
@@ -465,7 +465,7 @@ Proof.
   destruct Hp as (Hstrs_eq & Hsnp_eq & Hsnc_eq & Hscs_eq & Hwf_s & Hwf_t & Hdom_eq).
   specialize (pool_safe_implies Hsafe Hpool) as (?&[= <-]&Hcall_in & trss' & Htrss).
   edestruct trees_equal_access_all_protected_initialized as (trst' & Htrst & Htrseq').
-  11: exact Hstrs_eq. 5,7: rewrite Hscs_eq. 11: exact Htrss. 1,3,4,7,8: by eapply Hwf_s. 4: rewrite Hsnp_eq Hsnc_eq. 1-4: by eapply Hwf_t. 1: done.
+  13: exact Hstrs_eq. 7,9: rewrite Hscs_eq. 13: exact Htrss. 1,4,6,9,10: by eapply Hwf_s. 6: rewrite Hsnp_eq Hsnc_eq. 1-6: by eapply Hwf_t. 1: done.
   iSplit.
   { iPureIntro. do 3 eexists. eapply end_call_base_step. all: by rewrite -Hscs_eq. }
   iIntros (e_t' efs_t σ_t') "%Hhead".
